proof/correctness/avx2/KyberPolyvec_avx2_proof.ec
@@ -30,29 +30,27 @@ import NTT_Avx2.
 import AVX2_cf.
 
 lemma polyvec_compress_corr _a (_p : address) mem :
-    equiv [ Mprevec.polyvec_compress ~ EncDec_AVX2.encode10 :
+    equiv [ Mprevec.polyvec_compress ~ EncDec_AVX2.encode10_opt_vec :
              pos_bound768_cxq a{1} 0 768 2 /\
-             lift_array768 a{1} = _a /\
-             p{2} = compress_polyvec 10 _a /\
-             valid_ptr _p 384 /\
+             lift_vector a{1} = _a /\
+             a{2} = compress_polyvec 10 _a /\
+             valid_ptr _p 960 /\
              Glob.mem{1} = mem /\ to_uint rp{1} = _p
               ==>
-             lift_array768 res{1} = _a /\
-             pos_bound768_cxq res{1} 0 768 1 /\
-             touches mem Glob.mem{1} _p 384 /\
-             load_array384 Glob.mem{1} _p = res{2}].
-admitted.
+             touches mem Glob.mem{1} _p 960 /\
+             load_array960 Glob.mem{1} _p = res{2}].
+admitted. (* Miguel *)
 
 lemma polyvec_decompress_corr mem _p (_a : W8.t Array384.t): 
-    equiv [ Mprevec.polyvec_decompress ~ EncDec_AVX2.decode10 :
-             valid_ptr _p 384 /\
+    equiv [ Mprevec.polyvec_decompress ~ EncDec_AVX2.decode10_opt_vec :
+             valid_ptr _p 320 /\
              Glob.mem{1} = mem /\ to_uint ap{1} = _p /\
-             load_array384 Glob.mem{1} _p = _a /\ a{2} = _a
+             load_array320 Glob.mem{1} _p = _a /\ a{2} = _a
               ==>
              Glob.mem{1} = mem /\
-             lift_array768 res{1} = decompress_poly 10 res{2} /\
+             lift_vector res{1} = decompress_polyvec 10 res{2} /\
              pos_bound768_cxq res{1} 0 768 1].
-admitted.
+admitted. (* Miguel *)
 
 
 lemma polvec_add_corr_h _a _b ab bb:
